Add aligned encoder and decoder for strings.

src/Narcissus/BinLib/AlignedString.v
@@ -19,17 +19,19 @@ Require Import
         Fiat.Narcissus.Formats.FixListOpt
         Fiat.Narcissus.Formats.SumTypeOpt
         Fiat.Narcissus.Formats.AsciiOpt
+        Fiat.Narcissus.Formats.WordOpt
         Fiat.Narcissus.BinLib.AlignedByteString
         Fiat.Narcissus.BinLib.AlignWord
         Fiat.Narcissus.BinLib.AlignedEncodeMonad
         Fiat.Narcissus.BinLib.AlignedDecodeMonad
+        Fiat.Narcissus.BinLib.AlignedList
         Fiat.Common.IterateBoundedIndex
         Fiat.Common.Tactics.CacheStringConstant.
 
 Require Import
         Bedrock.Word.
 
-Section AlignedList.
+Section AlignedString.
 
   Context {cache : Cache}.
   Context {cacheAddNat : CacheAdd cache nat}.
@@ -39,197 +41,132 @@ Section AlignedList.
 
   Variable addE_addE_plus :
     forall (ce : CacheFormat) (n m : nat), addE (addE ce n) m = addE ce (n + m).
+  Variable addE_0 :
+    forall (ce : CacheFormat), addE ce 0 = ce.
 
-  Definition asciiToWord (a : ascii) : word 8 :=
-    match a with
-    | Ascii b0 b1 b2 b3 b4 b5 b6 b7 =>WS b0 (WS b1 (WS b2 (WS b3 (WS b4 (WS b5 (WS b6 (WS b7 WO)))))))
-    end.
+  (* Definition asciiToWord (a : ascii) : word 8 := *)
+  (*   match a with *)
+  (*   | Ascii b0 b1 b2 b3 b4 b5 b6 b7 =>WS b0 (WS b1 (WS b2 (WS b3 (WS b4 (WS b5 (WS b6 (WS b7 WO))))))) *)
+  (*   end. *)
 
-  Fixpoint AlignedEncodeString'
-           (sz : nat)
-           v
-           idx
-           (s : string)
-           env
+  (* Lemma asciiToWord_eq : *)
+  (*   forall a, *)
+  (*     (NToWord 8 (N_of_ascii a)) = asciiToWord a. *)
+  (* Proof. *)
+  (*   destruct a; simpl. *)
+  (*   destruct b; destruct b0; destruct b1; destruct b2; *)
+  (*     destruct b3; destruct b4; destruct b5; destruct b6; *)
+  (*     simpl; eauto. *)
+  (* Qed. *)
+
+  (* Fixpoint AlignedEncodeString' *)
+  (*          (sz : nat) *)
+  (*          v *)
+  (*          idx *)
+  (*          (s : string) *)
+  (*          env *)
+  (*   : option (ByteBuffer.t sz * nat * CacheFormat) := *)
+  (*     match s with *)
+  (*     | EmptyString => if Coq.Init.Nat.ltb idx (S sz) then @ReturnAlignedEncodeM _ string sz v idx EmptyString env else None *)
+  (*     | String a s' => Ifopt (SetCurrentBytes (sz := 1) v idx (asciiToWord a) env) as a' Then *)
+  (*                                                               AlignedEncodeString' sz (fst (fst a')) *)
+  (*                                                             (snd (fst a')) *)
+  (*                                                             s' (snd a') *)
+  (*                                                             Else None *)
+  (*   end. *)
+
+  (* Definition AlignedEncodeString *)
+  (*   : forall sz, AlignedEncodeM (S := string) sz := AlignedEncodeString'. *)
+
+  (* TODO: the aligned encoder and decoder for string reduce to those for list
+  at the moment. We can (and should) write a more optimized (fused) version
+  later and show they are equivalent. *)
+  Definition list_word_of_string (s : string) : list (word 8) :=
+    map (fun a => NToWord 8 (N_of_ascii a)) (list_ascii_of_string s).
+
+  Definition string_of_list_word (l : list (word 8)) : string :=
+    string_of_list_ascii (map (fun w => ascii_of_N (wordToN w)) l).
+
+  Definition AlignedEncodeString'
+             (sz : nat) v idx (s : string) env
     : option (ByteBuffer.t sz * nat * CacheFormat) :=
-      match s with
-      | EmptyString => if Coq.Init.Nat.ltb idx (S sz) then @ReturnAlignedEncodeM _ string sz v idx EmptyString env else None
-      | String a s' => Ifopt (SetCurrentBytes (sz := 1) v idx (asciiToWord a) env) as a' Then
-                                                                AlignedEncodeString' sz (fst (fst a'))
-                                                              (snd (fst a'))
-                                                              s' (snd a')
-                                                              Else None
-    end.
-
-  Lemma asciiToWord_eq :
-    forall a,
-      (NToWord 8 (N_of_ascii a)) = asciiToWord a.
-  Proof.
-    destruct a; simpl.
-    destruct b; destruct b0; destruct b1; destruct b2;
-      destruct b3; destruct b4; destruct b5; destruct b6;
-      simpl; eauto.
-  Qed.
+    AlignedEncodeList (fun _ => SetCurrentBytes (sz:=1)) sz v idx
+                      (list_word_of_string s) env.
 
   Definition AlignedEncodeString
     : forall sz, AlignedEncodeM (S := string) sz := AlignedEncodeString'.
 
+  Definition AlignedDecodeString {m}
+             (n : nat)
+    : AlignedDecodeM string m :=
+    (l <- ListAlignedDecodeM (fun _ => GetCurrentByte) n;
+     return (string_of_list_word l))%AlignedDecodeM.
+
   Lemma CorrectAlignedEncoderForFormatString
     : CorrectAlignedEncoder format_string AlignedEncodeString.
   Proof.
-    unfold CorrectAlignedEncoder; intros.
-    eexists (fix EncodeString (s : string) env :=
-               match s with
-               | EmptyString => Some (mempty, env)
-               | String a s' => `(t1, env') <- Some (WordOpt.encode_word (asciiToWord a) env);
-                             `(t2, env'') <- EncodeString s' env';
-                             Some (mappend t1 t2, env'')
-               end); split; [ split | split ].
-    - revert env; induction s; intros; simpl; eauto.
-      + injections; reflexivity.
-      + simpl in H.
-        unfold Bind2.
-        unfold format_ascii.
-        unfold WordOpt.format_word; simpl.
-        destruct ((fix EncodeString (s : string) (env : CacheFormat) {struct s} :
-                            option (ByteString * CacheFormat) :=
-                          match s with
-                          | ""%string => Some (ByteString_id, env)
-                          | String a s' =>
-                              `(t2, env'') <- EncodeString s' (addE env 8);
-                              Some
-                                (ByteString_enqueue_ByteString
-                                   (WordOpt.encode_word' 8 (asciiToWord a) ByteString_id) t2, env'')
-                          end)) eqn: ?; simpl in H; try discriminate.
-        destruct p; injections.
-        rewrite refineEquiv_bind_unit, IHs, refineEquiv_bind_unit; eauto.
-        simpl; rewrite asciiToWord_eq.
-        reflexivity.
-    - revert env; induction s; intros; simpl; eauto; try discriminate.
-      simpl in H.
-      destruct ((fix EncodeString (s : string) (env : CacheFormat) {struct s} :
-                            option (ByteString * CacheFormat) :=
-                          match s with
-                          | ""%string => Some (ByteString_id, env)
-                          | String a s' =>
-                              `(t2, env'') <- EncodeString s' (addE env 8);
-                              Some
-                                (ByteString_enqueue_ByteString
-                                   (WordOpt.encode_word' 8 (asciiToWord a) ByteString_id) t2, env'')
-                          end)) eqn: ?; simpl in H; try discriminate.
-      destruct p; injections; try discriminate.
-      unfold Bind2.
-      unfold format_ascii.
-      intro; computes_to_inv.
-      unfold WordOpt.format_word in H0; computes_to_inv; subst.
-      eapply IHs; eauto.
-    - induction s; intros; simpl; eauto.
-      + injections; reflexivity.
-      + simpl in *.
-        destruct ((fix EncodeString (s : string) (env : CacheFormat) {struct s} :
-                     option (ByteString * CacheFormat) :=
-                     match s with
-                     | ""%string => Some (ByteString_id, env)
-                     | String a s' =>
-                       `(t2, env'') <- EncodeString s' (addE env 8);
-                       Some
-                         (ByteString_enqueue_ByteString
-                            (WordOpt.encode_word' 8 (asciiToWord a) ByteString_id) t2, env'')
-                     end)) eqn: ?; simpl in H; try discriminate.
-        destruct p; injections; try discriminate.
-        eapply IHs in Heqo.
-        erewrite padding_ByteString_enqueue_ByteString, Heqo.
-        destruct a; reflexivity.
-    - unfold EncodeMEquivAlignedEncodeM; intros.
-      generalize (le_refl (String.length s)); remember (String.length s) eqn: s_eq; rewrite s_eq at 1; clear s_eq.
-      revert s env idx. induction n; intros ? ? ? le_s.
-      + destruct s; simpl in le_s; try solve [inversion le_s].
-        repeat apply conj; intros.
-        * injections; simpl in v; pattern v; apply case0; simpl.
-          setoid_rewrite (proj2 (PeanoNat.Nat.ltb_lt idx (S idx + m))); try lia.
-          eexists _; split.
-          revert v1; rewrite <- (plus_n_O idx); intro; reflexivity.
-          pose proof mempty_left as H'; simpl in H'; rewrite H', build_aligned_ByteString_append;
-            reflexivity.
-        * injections; rewrite length_ByteString_ByteString_id in H0.
-          unfold AlignedEncodeString; simpl.
-          destruct (NPeano.Nat.ltb idx (S numBytes')) eqn: ?; eauto.
-          apply PeanoNat.Nat.ltb_lt in Heqb; lia.
-        * injections; simpl in H0; congruence.
-        * discriminate.
-      + destruct s; simpl in le_s; try solve [inversion le_s].
-        * repeat apply conj; intros.
-          -- injections; simpl in v; pattern v; apply case0; simpl.
-             setoid_rewrite (proj2 (PeanoNat.Nat.ltb_lt idx (S idx + m))); try Lia.lia.
-             eexists _; split.
-             revert v1; rewrite <- (plus_n_O idx); intro; reflexivity.
-             pose proof mempty_left as H'; simpl in H'; rewrite H', build_aligned_ByteString_append;
-               reflexivity.
-          -- injections; rewrite length_ByteString_ByteString_id in H0.
-             unfold AlignedEncodeString; simpl.
-             destruct (NPeano.Nat.ltb idx (S numBytes')) eqn: ?; eauto.
-             apply PeanoNat.Nat.ltb_lt in Heqb; lia.
-          -- injections; simpl in H0; congruence.
-          -- discriminate.
-        * apply le_S_n in le_s.
-          intuition.
-          simpl in H.
-          -- destruct ((fix EncodeString (s : string) (env : CacheFormat) {struct s} :
-                          option (ByteString * CacheFormat) :=
-                          match s with
-                          | ""%string => Some (ByteString_id, env)
-                          | String a s' =>
-                            `(t2, env'') <- EncodeString s' (addE env 8);
-                            Some
-                              (ByteString_enqueue_ByteString
-                                 (WordOpt.encode_word' 8 (asciiToWord a) ByteString_id) t2, env'')
-                          end)) eqn: ?; simpl in H; try discriminate.
-             destruct p; injections; try discriminate.
-             simpl in *.
-             eapply IHn in le_s.
-             intuition.
-             eapply H in Heqo.
-             destruct Heqo; intuition.
-             eexists _.
-             intuition.
-             (*unfold SetCurrentByte; simpl.
-             simpl.
+    eapply CorrectAlignedEncoder_morphism; cycle 1. reflexivity.
+    - unfold AlignedEncodeString, AlignedEncodeString'.
+      eapply CorrectAlignedEncoderForProjection_Format.
+      eapply CorrectAlignedEncoderForFormatList.
+      unshelve instantiate (2:=_).
+      eapply CorrectAlignedEncoderForFormatNChar; eauto.
+      intros; eapply encoder_format_eq_cache_OK; eauto.
+      simpl. intros ?????? H1 _ H2.
+      unfold format_word in H1. computes_to_inv.
+      inversion H1. inversion H2.
+      reflexivity.
+    - unfold FMapFormat.Projection_Format, FMapFormat.Compose_Format.
+      intros s env; split.
+      + intros v [?[??]]. subst.
+        revert dependent v. revert dependent env.
+        induction s; simpl; unfold Bind2; intros; eauto.
+        computes_to_inv.
+        computes_to_econstructor; eauto.
+        computes_to_econstructor; eauto using eq_ret_compute.
+      + intros v ?. rewrite unfold_computes.
+        revert dependent v. revert dependent env.
+        induction s; simpl; unfold Bind2; intros; eauto.
+        repeat esplit; eauto.
+        computes_to_inv.
+        apply IHs in H'. destruct_conjs.
+        inversion H''. subst.
+        repeat esplit.
+        simpl.
+        computes_to_econstructor; eauto.
+        computes_to_econstructor; eauto.
+  Qed.
 
+  Lemma AlignedDecodeStringM {C : Type}
+        (n : nat)
+    : forall (t : string -> DecodeM (C * _) ByteString)
+             (t' : string -> forall {numBytes}, AlignedDecodeM C numBytes),
+      (forall b, DecodeMEquivAlignedDecodeM (t b) (@t' b))
+      -> DecodeMEquivAlignedDecodeM
+           (fun v cd => `(l, bs, cd') <- decode_string n v cd;
+                          t l bs cd')
+           (fun numBytes => l <- AlignedDecodeString n;
+                            t' l)%AlignedDecodeM.
+  Proof.
+    intros.
+    unfold AlignedDecodeString.
+    eapply Bind_DecodeMEquivAlignedDecodeM; eauto.
+    eapply DecodeMEquivAlignedDecodeM_trans.
+    3: intros; apply AlignedDecodeMEquiv_refl.
+    - eapply AlignedDecodeListM.
+      apply AlignedDecodeCharM.
+      intros; eapply Return_DecodeMEquivAlignedDecodeM.
+    - simpl. clear.
+      induction n; intros; simpl; eauto.
+      unfold decode_ascii.
+      rewrite !DecodeBindOpt2_assoc.
+      eapply DecodeBindOpt2_under_bind; intros; simpl.
+      rewrite <- IHn.
+      rewrite !DecodeBindOpt2_assoc.
+      eapply DecodeBindOpt2_under_bind; intros; simpl.
+      reflexivity.
+  Qed.
 
-             simpl in H2.
-          eapply H.
-          assert ((forall (s : A * {As : list A & le (length As) n} ) (env : CacheFormat) (t : ByteString) (env' : CacheFormat),
-                      (projT1 X ∘ fst) s env = Some (t, env') -> padding t = 0)) as H'.
-          { destruct X; clear IHn; simpl in *; intuition eauto. }
-          assert (EncodeMEquivAlignedEncodeM (projT1 X ∘ fst)
-                                             (fun (sz : nat) (t : ByteBuffer.t sz) (idx : nat)
-                                                  (s : A * {As : list A & le (length As) n})
-                                                  (env : CacheFormat) => encode_A sz t idx (fst s) env)) as H''.
-          { destruct X; clear IHn; simpl in *; intuition eauto.
-            unfold EncodeMEquivAlignedEncodeM; intros ? [? ?] ?; unfold Basics.compose; simpl.
-            apply H2; eauto. }
-          assert (EncodeMEquivAlignedEncodeM (S := A * {As : list A & le (length As) n})
-                    ((fix AlignedEncodeList (As : list A)
-                          (env : CacheFormat) {struct As} : option (ByteString * CacheFormat) :=
-                        match As with
-                        | [] => Some (mempty, env)
-                        | a :: As' => `(t1, env') <- projT1 X a env;
-                                      `(t2, env'') <- AlignedEncodeList As' env';
-                                      Some (mappend t1 t2, env'')
-                        end) ∘ (@projT1 _ _) ∘ snd )
-                    (fun (sz : nat) (t : ByteBuffer.t sz) (idx : nat)
-                         (s : A * {As : list A & le (length As) n}) (env : CacheFormat) =>
-                       AlignedEncodeList encode_A sz t idx (projT1 (snd s)) env)) as H'''.
-          { unfold EncodeMEquivAlignedEncodeM; intros ? [? [? ?] ] ?; simpl; eauto. }
-          apply le_S_n in le_s.
-        pose proof (Append_EncodeMEquivAlignedEncodeM _
-                                                      _
-                                                      _
-                                                      _
-                                                      H' H'' H''' env (a, existT _ s le_s) idx); clear H' H'' H'''.
-        intuition.
-  Qed. *)
-  Admitted.
 
   Lemma CorrectAlignedEncoderForFormatStringTerm
         term_char
@@ -263,7 +200,7 @@ Section AlignedList.
     apply (projT2 (CorrectAlignedEncoderForFormatStringTerm _)).
   Qed.
 
-  Fixpoint StringAlignedDecodeM {m}
+  Fixpoint StringTermAlignedDecodeM {m}
            (term_char : word 8)
            (n : nat)
     : AlignedDecodeM string m :=
@@ -272,11 +209,11 @@ Section AlignedList.
     | S n' => BindAlignedDecodeM GetCurrentByte
                                  (fun c => if (weqb c term_char)
                                            then ReturnAlignedDecodeM EmptyString
-                                           else BindAlignedDecodeM (StringAlignedDecodeM term_char n')
+                                           else BindAlignedDecodeM (StringTermAlignedDecodeM term_char n')
                                                                    (fun s => ReturnAlignedDecodeM (String (ascii_of_N (wordToN c)) s)))
     end%AlignedDecodeM%list.
 
-  Lemma AlignedDecodeStringM {C : Type}
+  Lemma AlignedDecodeStringTermM {C : Type}
         (term_word : word 8)
         (term_char : ascii)
     : forall (t : string -> DecodeM (C * _) ByteString)
@@ -286,7 +223,7 @@ Section AlignedList.
       -> DecodeMEquivAlignedDecodeM
            (fun v cd => `(l, bs, cd') <- decode_string_with_term_char term_char v cd;
                           t l bs cd')
-           (fun numBytes => l <- @StringAlignedDecodeM numBytes term_word numBytes;
+           (fun numBytes => l <- @StringTermAlignedDecodeM numBytes term_word numBytes;
            t' l)%AlignedDecodeM%list.
   Proof.
     intros.
@@ -316,4 +253,4 @@ Section AlignedList.
     eapply H0. *)
   Admitted.
 
-End AlignedList.
+End AlignedString.
